@prefix xsd: <http://www.w3.org/2001/XMLSchema#> .
@prefix owl: <http://www.w3.org/2002/07/owl#> .
@prefix vs: <http://www.w3.org/2003/06/sw-vocab-status/ns#> .
@prefix : <http://geovocab.org/geometry#> .
@prefix xml: <http://www.w3.org/XML/1998/namespace> .
@prefix rdf: <http://www.w3.org/1999/02/22-rdf-syntax-ns#> .
@prefix rdfs: <http://www.w3.org/2000/01/rdf-schema#> .
@prefix skos: <http://www.w3.org/2004/02/skos/core#> .
@prefix geo: <http://www.w3.org/2003/01/geo/wgs84_pos#> .
@base <http://geovocab.org/geometry> .

<http://geovocab.org/geometry> rdf:type owl:Ontology ;
                               
                               rdfs:label "NeoGeo Geometry Ontology" ;

			       owl:imports <http://geovocab.org/mappings/geometry> ;
                               
                               rdfs:comment "A vocabulary for describing geographical regions in RDF. $Id: geometry.ttl 97 2012-04-16 12:46:18Z jmsalas@gmail.com $" .


#################################################################
#
#    Annotation properties
#
#################################################################


vs:term_status rdf:type owl:AnnotationProperty .



#################################################################
#
#    Classes
#
#################################################################


###  Geometry

:Geometry rdf:type owl:Class ;
          
          rdfs:label "Geometry" ;
          
          vs:term_status "testing" ;
          
          rdfs:comment "Super-class grouping all geometrical representations (also ones in non-RDF formats, such as KML, GML, WKT...)." .



###  GeometryCollection

:GeometryCollection rdf:type owl:Class ;
                    
                    rdfs:label "Geometry Collection" ;
                    
                    rdfs:subClassOf :Geometry ;
                    
                    vs:term_status "unstable" ;
                    
                    rdfs:comment "Super-class grouping all composite geometrical representations." .


###  Bounding Box

:BoundingBox rdf:type owl:Class ;
            
             rdfs:label "Bounding Box" ;
            
             rdfs:subClassOf :Geometry ;
            
             rdfs:comment "Represents a bounding box composed by four line segments." ;
            
             vs:term_status "unstable" .


###  LineString

:LineString rdf:type owl:Class ;
            
            rdfs:label "LineString" ;
            
            rdfs:subClassOf :Geometry ;
            
            rdfs:comment "Represents a series of points connected by straight lines." ;
            
            vs:term_status "unstable" .



###  LinearRing

:LinearRing rdf:type owl:Class ;
            
            rdfs:label "LinearRing" ;
            
            rdfs:subClassOf :LineString ;
            
            vs:term_status "unstable" ;
            
            rdfs:comment "Represents a series of points connected by straight lines, which form a closed shape. Last point must be the same as the first point." .



###  MultiLineString

:MultiLineString rdf:type owl:Class ;
                 
                 rdfs:label "MultiLineString" ;
                 
                 rdfs:subClassOf :GeometryCollection ;
                 
                 vs:term_status "unstable" ;
                 
                 rdfs:comment "Describes a geometric shape composed of several LineString resources." .



###  MultiPoint

:MultiPoint rdf:type owl:Class ;
            
            rdfs:label "MultiPoint" ;
            
            rdfs:subClassOf :GeometryCollection ;
            
            rdfs:comment "Describes a collection of Point resources, which define a resource's geometric representation." ;
            
            vs:term_status "unstable" .



###  MultiPolygon

:MultiPolygon rdf:type owl:Class ;
              
              rdfs:label "MultiPolygon" ;
              
              rdfs:subClassOf :GeometryCollection ;
              
              vs:term_status "unstable" ;
              
              rdfs:comment "Describes a geometric shape composed of several Polygon resources." .



###  Polygon

:Polygon rdf:type owl:Class ;
         
         rdfs:label "Polygon" ;
         
         rdfs:subClassOf :Geometry ,
                                                          [ rdf:type owl:Restriction ;
                                                            owl:onProperty :exterior ;
                                                            owl:onClass :LinearRing ;
                                                            owl:qualifiedCardinality "1"^^xsd:nonNegativeInteger
                                                          ] ,
                                                          [ rdf:type owl:Restriction ;
                                                            owl:onProperty :interior ;
                                                            owl:someValuesFrom :LinearRing
                                                          ] ;
         
         rdfs:comment "A closed area defined by an exterior boundary, and optionally one or more interior boundaries." ;
         
         vs:term_status "unstable" .



###  http://www.w3.org/2003/01/geo/wgs84_pos#Point

geo:Point rdf:type owl:Class ;
                                               
                                               rdfs:label "Point" .



#################################################################
#
#    Object Properties
#
#################################################################


###  boundary

:boundary rdf:type owl:ObjectProperty ;
          
          rdfs:label "boundary" ;
          
          vs:term_status "unstable" ;
          
          rdfs:comment "Super-property that groups all properties defining a polygon's boundaries." ;
          
          rdfs:range :LinearRing ;
          
          rdfs:domain :Polygon .



###  exterior

:exterior rdf:type owl:ObjectProperty ;
          
          rdfs:label "exterior" ;
          
          rdfs:comment "Defines a polygon's outer boundary." ;
          
          vs:term_status "unstable" ;
          
          rdfs:range :LinearRing ;
          
          rdfs:domain :Polygon ;
          
          rdfs:subPropertyOf :boundary .



###  geometry

:geometry rdf:type owl:ObjectProperty ;
          
          rdfs:label "geometry" ;
          
          vs:term_status "testing" ;
          
          rdfs:comment "Relates a resource to its geometric shape." ;
          
          rdfs:range :Geometry .



###  interior

:interior rdf:type owl:ObjectProperty ;
          
          rdfs:label "interior" ;
          
          rdfs:comment "Defines an polygon's boundary within its outer boundary, i.e. a polygon with 'holes' in it." ;
          
          vs:term_status "unstable" ;
          
          rdfs:range :LinearRing ;
          
          rdfs:domain :Polygon ;
          
          rdfs:subPropertyOf :boundary .



###  lineStringMember

:lineStringMember rdf:type owl:ObjectProperty ;
                  
                  rdfs:label "LineString member" ;
                  
                  vs:term_status "unstable" ;
                  
                  rdfs:comment "Links a LineString simple geometry to a MultiLineString composite geometry." ;
                  
                  rdfs:range :LineString ;
                  
                  rdfs:domain :MultiLineString .



###  partOf

:partOf rdf:type owl:ObjectProperty ;
        
        rdfs:label "part of" ;
        
        vs:term_status "unstable" ;
        
        rdfs:comment "Relates a point to a geometric shape's boundary." ;
        
        rdfs:range :LineString ;
        
        rdfs:domain geo:Point .



###  pointMember

:pointMember rdf:type owl:ObjectProperty ;
             
             rdfs:label "Point member" ;
             
             rdfs:comment "Links a Point simple geometry to a MultiPoint composite Geometry." ;
             
             vs:term_status "unstable" ;
             
             rdfs:domain :MultiPoint ;
             
             rdfs:range geo:Point .



###  polygonMember

:polygonMember rdf:type owl:ObjectProperty ;
               
               rdfs:label "Polygon member" ;
               
               vs:term_status "unstable" ;
               
               rdfs:comment "Links a Polygon simple geometry to a MultiPolygon composite geometry." ;
               
               rdfs:domain :MultiPolygon ;
               
               rdfs:range :Polygon .



###  posList

:posList rdf:type owl:ObjectProperty ;
         
         rdfs:label "position list" ;
         
         rdfs:comment "Relates a LineString or LinearRing to the points that define them." ;
         
         vs:term_status "unstable" ;
         
         rdfs:domain :LineString .


###  bbox

:bbox rdf:type owl:ObjectProperty ;
         
      rdfs:label "bounding box" ;
         
      rdfs:comment "Relates a Geometry to its Bounding Box." ;
         
      vs:term_status "unstable" ;
         
      rdfs:domain :Geometry ;

      rdfs:range :BoundingBox .





#################################################################
#
#    Data properties
#
#################################################################


###  http://geovocab.org/geometry#asWKT

:asWKT rdf:type owl:DatatypeProperty ;
                                    
       rdfs:label "As WKT" ;
                                    
       rdfs:comment "WKT serialization of the geometry." ;
                                    
       vs:term_status "deprecated" .


###  http://geovocab.org/geometry#resolution

:resolution rdf:type owl:DatatypeProperty ;
                                    
       rdfs:label "Resolution" ;
                                    
       rdfs:comment "Resolution of the represented geometry object (expressed in meters)." ;
                                    
       vs:term_status "unstable" .

###  Generated by the OWL API (version 3.2.3.22702) http://owlapi.sourceforge.net

